operator overloading allows us to get rid of `Definition sepcl`

bedrock2/src/bedrock2/OperatorOverloading.v
@@ -28,17 +28,49 @@ Class PointsTo{width: Z}{word: word.word width}{mem: map.map word Byte.byte}{V: 
 (* Precedence: `*` is at level 40, and we want to bind stronger than `*`, and moreover,
    `^` is at level 30, and for consistency, we also want to bind stronger than `^`,
    so we choose 25. *)
-Notation "a |-> v" := (infer! PointsTo a v)
-  (at level 25, only parsing).
+Notation "a ~> v" := (infer! PointsTo a v)
+  (at level 25, only parsing) : oo_scope.
 
-#[export] Instance PointsToScalar{width}{word: word.word width}{mem: map.map word Byte.byte}
- (a v: word): PointsTo a v (scalar a v) := {}.
+Class PointsToPredicate{width}{word: word.word width}{mem: map.map word Byte.byte}
+      (V: Type)(pred: word -> V -> mem -> Prop) := {}.
 
-Notation "a |-> v" := (scalar a v)
-  (at level 25, format "'[  ' a  |->  '/' v ']'", only printing).
+#[export] Instance PointsToPredicate_to_PointsTo
+ {width}{word: word.word width}{mem: map.map word Byte.byte}{V: Type}
+ (pred: word -> V -> mem -> Prop){p: PointsToPredicate V pred}
+ (a: word)(v: V): PointsTo a v (pred a v) := {}.
+
+#[export] Instance PointsToScalarPredicate
+ {width}{word: word.word width}{mem: map.map word Byte.byte}:
+  PointsToPredicate word scalar := {}.
+Notation "a ~> v" := (scalar a v)
+  (at level 25, format "'[  ' a  ~>  '/' v ']'", only printing) : oo_scope.
+
+Class PredicateSize{width}{word: word.word width}{mem: map.map word Byte.byte}{V: Type}
+      (pred: word -> V -> mem -> Prop){p: PointsToPredicate V pred}(sz: Z) := {}.
+
+#[export] Instance Scalar32Size{word: word.word 32}{mem: map.map word Byte.byte}:
+  PredicateSize (scalar (word := word)) 4 | 5 := {}.
+#[export] Instance Scalar64Size{word: word.word 64}{mem: map.map word Byte.byte}:
+  PredicateSize (scalar (word := word)) 8 | 5 := {}.
+#[export] Instance ScalarGenericSize
+ {width: Z}{word: word.word width}{mem: map.map word Byte.byte}:
+  PredicateSize (scalar (word := word)) (Memory.bytes_per_word width) | 6 := {}.
+
 
 Require Import bedrock2.Array.
 
+Class PointsToArray{width}{word: word.word width}{mem: map.map word Byte.byte}{V: Type}
+      (a: word)(vs: list V)(pred: mem -> Prop) := {}.
+Notation "a --> vs" := (infer! PointsToArray a vs)
+  (at level 25, only parsing) : oo_scope.
+Notation "a --> vs" := (array _ _ a vs)
+  (at level 25, format "'[  ' a  -->  '/' vs ']'", only printing) : oo_scope.
+
+#[export] Instance DerivePointsToArray
+ {width: Z}{word: word.word width}{mem: map.map word Byte.byte}{V: Type}
+ (a: word)(vs: list V)(elem: word -> V -> mem -> Prop){p: PointsToPredicate V elem}
+ (sz: Z){s: PredicateSize elem sz}:
+  PointsToArray a vs (array elem (word.of_Z sz) a vs) := {}.
 
 Section TestNotations.
   Context {width: Z} {word: word.word width} {mem: map.map word Byte.byte}.
@@ -52,19 +84,29 @@ Section TestNotations.
   Goal forall (P Q R: mem -> Prop), P * Q * R = sep (sep P Q) R. intros. srefl. Abort.
 
   Goal forall (a1 a2 ofs sz v1 v2: word) (R: mem -> Prop) (m: mem), (R * R) m. Abort.
-  Goal forall (a1 a2 ofs sz v1 v2: word) (R: mem -> Prop) (m: mem), (a1 |-> v1) m. Abort.
+  Goal forall (a1 a2 ofs sz v1 v2: word) (R: mem -> Prop) (m: mem), (a1 ~> v1) m. Abort.
   Goal forall (a1 a2 ofs sz v1 v2: word) (R: mem -> Prop) (m: mem),
-      (R * a1 |-> v1) m.
+      (R * a1 ~> v1) m.
   Abort.
   Goal forall (a1 a2 ofs sz v1 v2: word) (R: mem -> Prop) (m: mem),
-      ((a1 |-> v1) * R) m.
+      ((a1 ~> v1) * R) m.
   Abort.
   Goal forall (a1 a2 ofs sz v1 v2: word) (R: mem -> Prop) (m: mem),
-      (a1 |-> v1 * a2 |-> v2 * R) m.
+      (a1 ~> v1 * a2 ~> v2 * R) m.
     intros.
   Abort.
   Goal forall (a1 a2 ofs sz v1 v2: word) (R: mem -> Prop) (m: mem),
-      ((a1 + ofs * sz) |-> v1 * a2 |-> v2 * R) m.
+      ((a1 + ofs * sz) ~> v1 * a2 ~> v2 * R) m.
+    intros.
+  Abort.
+
+  Goal forall (a1 a2 ofs sz: word) (vs1 vs2: list word) (R: mem -> Prop) (m: mem),
+      ((a1 + ofs * sz) --> vs1 * a2 --> vs2 * R) m.
+    intros.
+  Abort.
+
+  Goal forall (a1 a2 ofs sz: word) (vs1 vs2: list word) (R: mem -> Prop) (m: mem),
+      ((a1 + ofs * sz) --> vs1 * a2 --> vs2[3 := word.of_Z (word := word) 1] * R) m.
     intros.
   Abort.
 End TestNotations.
